Knot proof with invariant style

examples/knot/Knot1.v
@@ -31,57 +31,51 @@ Section KNOT.
     Variable skenv: SkEnv.t.
 
     Definition rec_spec:    fspec :=
-      mk_simple (X:=(nat -> nat) * nat)
-                (fun '(f, n) => (
-                     (fun varg o =>
-                        (⌜varg = [Vint (Z.of_nat n)]↑ /\ o = ord_pure (2 * n + 1)%nat⌝)
-                          ** (OwnM (knot_frag (Some f)))
-                          ** inv_closed
-                     ),
-                     (fun vret =>
-                        (⌜vret = (Vint (Z.of_nat (f n)))↑⌝)
-                          ** (Own (GRA.embed (knot_frag (Some f))))
-                          ** inv_closed
-                     )
-                )).
+      mk_inv_simple (X:=(nat -> nat) * nat)
+                    (fun '(f, n) => (
+                         (fun varg o =>
+                            (⌜varg = [Vint (Z.of_nat n)]↑ /\ o = ord_pure (2 * n + 1)%nat⌝)
+                              ** (OwnM (knot_frag (Some f)))
+                         ),
+                         (fun vret =>
+                            (⌜vret = (Vint (Z.of_nat (f n)))↑⌝)
+                              ** (Own (GRA.embed (knot_frag (Some f))))
+                         )
+                    )).
 
     Definition fun_gen (f: nat -> nat): ftspec (list val) (val) :=
-      mk_simple (X:=nat)
-                (fun n => (
-                     (fun varg o =>
-                        (⌜exists fb,
-                              varg = [Vptr fb 0; Vint (Z.of_nat n)]↑ /\ o = ord_pure (2 * n)%nat /\
-                              fb_has_spec skenv (RecStb skenv) fb rec_spec⌝)
-                          ** OwnM (knot_frag (Some f))
-                          ** inv_closed
-                     ),
-                     (fun vret =>
-                        (⌜vret = (Vint (Z.of_nat (f n)))↑⌝)
-                          ** OwnM (knot_frag (Some f))
-                          ** inv_closed
-                     )
-                )).
+      mk_inv_simple (X:=nat)
+                    (fun n => (
+                         (fun varg o =>
+                            (⌜exists fb,
+                                  varg = [Vptr fb 0; Vint (Z.of_nat n)]↑ /\ o = ord_pure (2 * n)%nat /\
+                                  fb_has_spec skenv (RecStb skenv) fb rec_spec⌝)
+                              ** OwnM (knot_frag (Some f))
+                         ),
+                         (fun vret =>
+                            (⌜vret = (Vint (Z.of_nat (f n)))↑⌝)
+                              ** OwnM (knot_frag (Some f))
+                         )
+                    )).
 
     Definition KnotRecStb: list (gname * fspec) := [("rec", rec_spec)].
 
     Definition knot_spec:    fspec :=
-      mk_simple (X:=(nat -> nat))
-                (fun f => (
-                     (fun varg o =>
-                        (⌜exists fb,
-                              varg = [Vptr fb 0]↑ /\ o = ord_pure 1 /\
-                              fb_has_spec skenv (FunStb skenv) fb (fun_gen f)⌝)
-                          ** (∃ old, OwnM (knot_frag old))
-                          ** inv_closed
-                     ),
-                     (fun vret =>
-                        (⌜exists fb,
-                              vret = (Vptr fb 0)↑ /\
-                              fb_has_spec skenv (RecStb skenv) fb rec_spec⌝)
-                          ** OwnM (knot_frag (Some f))
-                          ** inv_closed
-                     )
-                )).
+      mk_inv_simple (X:=(nat -> nat))
+                    (fun f => (
+                         (fun varg o =>
+                            (⌜exists fb,
+                                  varg = [Vptr fb 0]↑ /\ o = ord_pure 1 /\
+                                  fb_has_spec skenv (FunStb skenv) fb (fun_gen f)⌝)
+                              ** (∃ old, OwnM (knot_frag old))
+                         ),
+                         (fun vret =>
+                            (⌜exists fb,
+                                  vret = (Vptr fb 0)↑ /\
+                                  fb_has_spec skenv (RecStb skenv) fb rec_spec⌝)
+                              ** OwnM (knot_frag (Some f))
+                         )
+                    )).
 
     Definition knot_spec2:    fspec :=
       mk_simple (X:=(nat -> nat))
@@ -91,7 +85,7 @@ Section KNOT.
                               varg = [Vptr fb 0]↑ /\ o = ord_pure 1 /\
                               fb_has_spec skenv (FunStb skenv) fb (fun_gen f)⌝)
                           ** OwnM (knot_init)
-                          ** inv_closed
+                          ** inv_opener
                      ),
                      (fun vret =>
                         (∃ INV,
@@ -110,7 +104,7 @@ Section KNOT.
     Definition SKnotSem: SModSem.t := {|
       SModSem.fnsems := KnotSbtb;
       SModSem.mn := "Knot";
-      SModSem.initial_mr := (GRA.embed (var_points_to skenv "_f" Vundef)) ⋅ (GRA.embed (knot_full None)) ⋅ (GRA.embed inv_black);
+      SModSem.initial_mr := (GRA.embed (inv_black tt↑ tt ↑)) ⋅ (GRA.embed (var_points_to skenv "_f" Vundef)) ⋅ (GRA.embed (knot_full None)) ;
       SModSem.initial_st := tt↑;
     |}
     .
@@ -131,13 +125,13 @@ Section WEAK.
   Context `{@GRA.inG invRA Σ}.
   Context `{@GRA.inG knotRA Σ}.
 
-  Lemma rec_spec_weaker f: ftspec_weaker (mrec_spec f (OwnM (knot_frag (Some f)) ** inv_closed)) rec_spec.
+  Lemma rec_spec_weaker f: ftspec_weaker (mrec_spec f (OwnM (knot_frag (Some f)) ** inv_opener)) rec_spec.
   Proof.
     ii. ss. exists (f, x_src). split.
     { intros arg_src arg_tgt o. ss.
       iIntros "[[H0 [H1 H2]] H3]". iModIntro. iFrame. }
     { intros ret_src ret_tgt. ss.
-      iIntros "[[[H0 H1] H2] H3]". iModIntro. iFrame. }
+      iIntros "[[H0 [H1 H2]] H3]". iModIntro. iFrame. }
   Qed.
 End WEAK.
 
@@ -156,9 +150,9 @@ Section WEAK.
       iIntros "[[[H0 H1] H2] H3]". iModIntro.
       iFrame. iExists (None: option (nat -> nat)). ss. }
     { intros ret_src ret_tgt.
-      iIntros "[[[H0 H1] H2] H3]". iModIntro. iFrame.
-      iExists (OwnM (knot_frag (Some x_src)) ** inv_closed).
-      iFrame. iDestruct "H0" as "%". iPureIntro. des. eexists.
+      iIntros "[[H0 [H1 H2]] H3]". iModIntro. iFrame.
+      iExists (OwnM (knot_frag (Some x_src)) ** inv_opener).
+      iFrame. iDestruct "H1" as "%". iPureIntro. des. eexists.
       split; eauto. eapply fb_has_spec_weaker; eauto.
       eapply rec_spec_weaker.
     }
