examples/mutsum/MutMain01proof.v
@@ -32,7 +32,7 @@ Section SIMMODSEM.
   Let W: Type := ((Σ * Any.t)) * ((Σ * Any.t)).
 
   Let wf: W -> Prop :=
-    mk_wf (fun (_: unit) => (True: iProp)%I) top2 top3.
+    mk_wf (fun (_: unit) _ _ => (True: iProp)%I) top4.
 
   Theorem correct: ModPair.sim MutMain1.Main MutMain0.Main.
   Proof.
